DynamoDbEncryption/dafny/StructuredEncryption/src/Canonize.dfy
@@ -1,0 +1,687 @@
+// Copyright Amazon.com Inc. or its affiliates. All Rights Reserved.
+// SPDX-License-Identifier: Apache-2.0
+include "../Model/AwsCryptographyDbEncryptionSdkStructuredEncryptionTypes.dfy"
+include "Util.dfy"
+include "Header.dfy"
+include "SortCanon.dfy"
+
+module Canonize {
+  import opened StructuredEncryptionUtil
+  import opened Types = AwsCryptographyDbEncryptionSdkStructuredEncryptionTypes
+  import opened Wrappers
+  import opened StandardLibrary
+  import opened StandardLibrary.UInt
+  import Header = StructuredEncryptionHeader
+  import Paths = StructuredEncryptionPaths
+  import SortCanon
+  import Relations
+
+  predicate method {:opaque} IsValidPath(path : Path)
+  {
+    Paths.ValidPath(path)
+  }
+
+  datatype EncryptionSelector = DoEncrypt | DoDecrypt
+
+  // Updated return true if the given item has been updated properly for the given operation.
+  // Updated2..Update5 do exactly the same thing, but with different data types.
+  predicate Updated(oldVal : CanonCryptoItem, newVal : CanonCryptoItem, mode : EncryptionSelector)
+  {
+    && oldVal.key == newVal.key
+    && oldVal.origKey == newVal.origKey
+    && oldVal.action == newVal.action
+    && (newVal.action != ENCRYPT_AND_SIGN <==> oldVal.data == newVal.data)
+    && (newVal.action == ENCRYPT_AND_SIGN <==> oldVal.data != newVal.data)
+    && (mode == DoEncrypt ==> (newVal.action == ENCRYPT_AND_SIGN ==> newVal.data.typeId == BYTES_TYPE_ID))
+    && (mode == DoDecrypt ==> (newVal.action == ENCRYPT_AND_SIGN ==> |oldVal.data.value| >= 2 && newVal.data.typeId == oldVal.data.value[..2]))
+  }
+
+  predicate Updated2(oldVal : AuthItem, newVal : CanonCryptoItem, mode : EncryptionSelector)
+  {
+    && oldVal.key == newVal.origKey
+    && (newVal.action != ENCRYPT_AND_SIGN <==> oldVal.data == newVal.data)
+    && (newVal.action == ENCRYPT_AND_SIGN <==> oldVal.data != newVal.data)
+    && (mode == DoEncrypt ==> (newVal.action == ENCRYPT_AND_SIGN ==> newVal.data.typeId == BYTES_TYPE_ID))
+    && (mode == DoDecrypt ==> (newVal.action == ENCRYPT_AND_SIGN ==> |oldVal.data.value| >= 2 && newVal.data.typeId == oldVal.data.value[..2]))
+  }
+
+  predicate Updated3(oldVal : AuthItem, newVal : CryptoItem, mode : EncryptionSelector)
+  {
+    && oldVal.key == newVal.key
+    && (newVal.action != ENCRYPT_AND_SIGN <==> oldVal.data == newVal.data)
+    && (newVal.action == ENCRYPT_AND_SIGN <==> oldVal.data != newVal.data)
+    && (mode == DoEncrypt ==> (newVal.action == ENCRYPT_AND_SIGN ==> newVal.data.typeId == BYTES_TYPE_ID))
+    && (mode == DoDecrypt ==> (newVal.action == ENCRYPT_AND_SIGN ==> |oldVal.data.value| >= 2 && newVal.data.typeId == oldVal.data.value[..2]))
+  }
+
+  predicate Updated4(oldVal : CryptoItem, newVal : CryptoItem, mode : EncryptionSelector)
+  {
+    && oldVal.key == newVal.key
+    && oldVal.action == newVal.action
+    && (newVal.action != ENCRYPT_AND_SIGN <==> oldVal.data == newVal.data)
+    && (newVal.action == ENCRYPT_AND_SIGN <==> oldVal.data != newVal.data)
+    && (mode == DoEncrypt ==> (newVal.action == ENCRYPT_AND_SIGN ==> newVal.data.typeId == BYTES_TYPE_ID))
+    && (mode == DoDecrypt ==> (newVal.action == ENCRYPT_AND_SIGN ==> |oldVal.data.value| >= 2 && newVal.data.typeId == oldVal.data.value[..2]))
+  }
+
+  predicate Updated5(oldVal : CryptoItem, newVal : CanonCryptoItem, mode : EncryptionSelector)
+  {
+    && oldVal.key == newVal.origKey
+    && oldVal.action == newVal.action
+    && (newVal.action != ENCRYPT_AND_SIGN <==> oldVal.data == newVal.data)
+    && (newVal.action == ENCRYPT_AND_SIGN <==> oldVal.data != newVal.data)
+    && (mode == DoEncrypt ==> (newVal.action == ENCRYPT_AND_SIGN ==> newVal.data.typeId == BYTES_TYPE_ID))
+    && (mode == DoDecrypt ==> (newVal.action == ENCRYPT_AND_SIGN ==> |oldVal.data.value| >= 2 && newVal.data.typeId == oldVal.data.value[..2]))
+  }
+
+  predicate method {:opaque} IsCanonPath(table : GoodString, origKey : Path, key : CanonicalPath)
+    requires IsValidPath(origKey)
+  {
+    reveal IsValidPath();
+    key == Paths.CanonPath(table, origKey)
+  }
+
+  function method {:opaque} MakeCanon(tableName : GoodString, data : CryptoItem) : (result : CanonCryptoItem)
+    requires Paths.ValidPath(data.key)
+    requires IsValidPath(data.key)
+    ensures result.origKey == data.key
+    ensures result.data == data.data
+    ensures result.action == data.action
+    ensures IsValidPath(result.origKey)
+    ensures result.key == Paths.CanonPath(tableName, data.key)
+    ensures IsCanonPath(tableName, data.key, result.key)
+    ensures IsCanonPath(tableName, result.origKey, result.key)
+  {
+    reveal IsValidPath();
+    reveal IsCanonPath();
+    CanonCryptoItem(Paths.CanonPath(tableName, data.key), data.key, data.data, data.action)
+  }
+
+  function method {:opaque} MakeCanonAuth(tableName : GoodString, data : AuthItem) : (result : CanonAuthItem)
+    requires Paths.ValidPath(data.key)
+    requires IsValidPath(data.key)
+    ensures result.origKey == data.key
+    ensures result.data == data.data
+    ensures result.action == data.action
+    ensures IsValidPath(result.origKey)
+    ensures result.key == Paths.CanonPath(tableName, data.key)
+    ensures IsCanonPath(tableName, data.key, result.key)
+    ensures IsCanonPath(tableName, result.origKey, result.key)
+  {
+    reveal IsValidPath();
+    reveal IsCanonPath();
+    CanonAuthItem(Paths.CanonPath(tableName, data.key), data.key, data.data, data.action)
+  }
+
+  predicate method Same(x : CanonAuthItem, y : CanonCryptoItem)
+  {
+    && x.key == y.key
+    && x.origKey == y.origKey
+    && x.data == y.data
+  }
+
+  function method MakeCryptoItem(x : CanonAuthItem, action : CryptoAction) : (ret : CanonCryptoItem)
+    ensures Same(x, ret)
+  {
+    CanonCryptoItem(x.key, x.origKey, x.data, action)
+  }
+
+  function method {:opaque} LegendToAction(v : Header.LegendByte) : CryptoAction
+  {
+    if v == Header.ENCRYPT_AND_SIGN_LEGEND then
+      ENCRYPT_AND_SIGN
+    else if v == Header.SIGN_AND_INCLUDE_IN_ENCRYPTION_CONTEXT_LEGEND then
+      SIGN_AND_INCLUDE_IN_ENCRYPTION_CONTEXT
+    else
+      SIGN_ONLY
+  }
+
+  function method {:tailrecursion} {:opaque} ResolveLegend(
+    fields : CanonAuthList,
+    legend : Header.Legend,
+    ghost origFields : CanonAuthList,
+    acc : CanonCryptoList
+  )
+    : (ret : Result<CanonCryptoList, Error>)
+    requires |fields| + |acc| == |origFields|
+    requires forall i | 0 <= i < |acc| :: Same(origFields[i], acc[i])
+    requires forall i | |acc| <= i < |origFields| :: origFields[i] == fields[i-|acc|]
+    ensures ret.Success? ==>
+              && |origFields| == |ret.value|
+              && forall i | 0 <= i < |origFields| :: Same(origFields[i], ret.value[i])
+  {
+    if |fields| == 0 then
+      :- Need(|legend| == 0, E("Schema changed : something that was signed is now unsigned."));
+      Success(acc)
+    else if fields[0].action == DO_NOT_SIGN then
+      ResolveLegend(fields[1..], legend, origFields, acc + [MakeCryptoItem(fields[0], DO_NOTHING)])
+    else
+      :- Need(0 < |legend|, E("Schema changed : something that was unsigned is now signed."));
+      ResolveLegend(fields[1..], legend[1..], origFields, acc + [MakeCryptoItem(fields[0], LegendToAction(legend[0]))])
+  }
+
+  function method {:opaque} ForEncrypt(tableName : GoodString, data : CryptoList)
+    : (ret : Result<CanonCryptoList, Error>)
+    requires CryptoListHasNoDuplicates(data)
+    ensures ret.Success? ==>
+              && CanonCryptoMatchesCryptoList(tableName, data, ret.value)
+              && IsCryptoSorted(ret.value)
+  {
+    :- Need(forall k <- data :: IsValidPath(k.key), E("Invalid Paths"));
+    var canonList := CryptoToCanonCrypto(tableName, data);
+    Success(CryptoSort(canonList, tableName, data))
+  }
+
+  predicate {:opaque} AuthExistsInCanonAuth(k : AuthItem, list : CanonAuthList)
+  {
+    exists x :: x in list && k.key == x.origKey && k.data == x.data
+  }
+
+  predicate {:opaque} AuthExistsInCrypto(k : AuthItem, list : CryptoList)
+  {
+    exists x :: x in list && k.key == x.key // && k.data == x.data
+  }
+
+  predicate {:opaque} CryptoExistsInAuth(k : CryptoItem, list : AuthList)
+  {
+    exists x :: x in list && k.key == x.key // && k.data == x.data
+  }
+
+  predicate {:opaque} AuthExistsInCanonCrypto(k : AuthItem, list : CanonCryptoList)
+  {
+    exists x :: x in list && k.key == x.origKey && k.data == x.data
+  }
+
+  predicate {:opaque} CryptoExistsInCanonCrypto(k : CryptoItem, list : CanonCryptoList)
+  {
+    exists x :: x in list && k.key == x.origKey && k.data == x.data
+  }
+
+  predicate {:opaque} CanonAuthExistsInAuth(k : CanonAuthItem, list : AuthList)
+  {
+    exists x :: x in list && k.origKey == x.key && k.data == x.data
+  }
+
+  predicate {:opaque} CanonCryptoExistsInAuth(k : CanonCryptoItem, list : AuthList)
+  {
+    exists x :: x in list && k.origKey == x.key && k.data == x.data
+  }
+
+  predicate {:opaque} CanonCryptoExistsInCrypto(k : CanonCryptoItem, list : CryptoList)
+  {
+    exists x :: x in list && k.origKey == x.key && k.data == x.data
+  }
+
+  predicate {:opaque} CanonAuthExistsInCanonAuth(k : CanonAuthItem, list : CanonAuthList)
+  {
+    exists x :: x in list && k.origKey == x.origKey && k.data == x.data
+  }
+
+  predicate {:opaque} CanonAuthExistsInCanonCrypto(k : CanonAuthItem, list : CanonCryptoList)
+  {
+    exists x :: x in list && k.origKey == x.origKey && k.data == x.data
+  }
+
+  predicate {:opaque} CanonCryptoExistsInCanonAuth(k : CanonCryptoItem, list : CanonAuthList)
+  {
+    exists x :: x in list && k.origKey == x.origKey && k.data == x.data
+  }
+
+  predicate {:opaque} CanonCryptoExistsInCanonCrypto(k : CanonCryptoItem, list : CanonCryptoList)
+  {
+    exists x :: x in list && k.origKey == x.origKey && k.data == x.data
+  }
+
+  predicate {:opaque} CanonAuthMatchesAuthList(tableName : GoodString, data : AuthList, canonList : CanonAuthList)
+  {
+    && (forall k <- data :: AuthExistsInCanonAuth(k, canonList))
+    && (forall k <- canonList :: CanonAuthExistsInAuth(k, data))
+    && |data| == |canonList|
+    && (forall k <- canonList :: IsValidPath(k.origKey))
+    && (forall k <- canonList :: IsCanonPath(tableName, k.origKey, k.key))
+    && CanonAuthListHasNoDuplicates(canonList)
+  }
+
+  predicate {:opaque} CanonCryptoMatchesAuthList(tableName : GoodString, data : AuthList, canonList : CanonCryptoList)
+  {
+    && (forall k <- data :: AuthExistsInCanonCrypto(k, canonList))
+    && (forall k <- canonList :: CanonCryptoExistsInAuth(k, data))
+    && |data| == |canonList|
+    && (forall k <- canonList :: IsValidPath(k.origKey))
+    && (forall k <- canonList :: IsCanonPath(tableName, k.origKey, k.key))
+    && CanonCryptoListHasNoDuplicates(canonList)
+  }
+
+  predicate {:opaque} CanonCryptoUpdatedAuth(k : CanonCryptoItem, list : AuthList)
+  {
+    exists x :: x in list && Updated2(x, k, DoDecrypt)
+  }
+
+  predicate {:opaque} AuthUpdatedCanonCrypto(k : AuthItem, list : CanonCryptoList)
+  {
+    exists x :: x in list && Updated2(k, x, DoDecrypt)
+  }
+
+  predicate {:opaque} CryptoUpdatedAuth(k : CryptoItem, list : AuthList)
+  {
+    exists x :: x in list && Updated3(x, k, DoDecrypt)
+  }
+
+  predicate {:opaque} AuthUpdatedCrypto(k : AuthItem, list : CryptoList)
+  {
+    exists x :: x in list && Updated3(k, x, DoDecrypt)
+  }
+
+  predicate {:opaque} CanonCryptoUpdatedCrypto(k : CanonCryptoItem, list : CryptoList)
+  {
+    exists x :: x in list && Updated5(x, k, DoDecrypt)
+  }
+
+  predicate {:opaque} CryptoUpdatedCanonCrypto(k : CryptoItem, list : CanonCryptoList)
+  {
+    exists x :: x in list && Updated5(k, x, DoDecrypt)
+  }
+
+  predicate {:opaque} NewCryptoUpdatedCrypto(k : CryptoItem, list : CryptoList)
+  {
+    exists x :: x in list && Updated4(x, k, DoDecrypt)
+  }
+
+  predicate {:opaque} CryptoUpdatedNewCrypto(k : CryptoItem, list : CryptoList)
+  {
+    exists x :: x in list && Updated4(k, x, DoDecrypt)
+  }
+
+  predicate {:opaque} CanonCryptoUpdatedAuthList(tableName : GoodString, data : AuthList, canonList : CanonCryptoList)
+  {
+    && (forall k <- data :: AuthUpdatedCanonCrypto(k, canonList))
+    && (forall k <- canonList :: CanonCryptoUpdatedAuth(k, data))
+    && |data| == |canonList|
+    && (forall k <- canonList :: IsValidPath(k.origKey))
+    && (forall k <- canonList :: IsCanonPath(tableName, k.origKey, k.key))
+    && CanonCryptoListHasNoDuplicates(canonList)
+  }
+
+  predicate {:opaque} CryptoUpdatedAuthList(data : AuthList, canonList : CryptoList)
+  {
+    && (forall k <- data :: AuthUpdatedCrypto(k, canonList))
+    && (forall k <- canonList :: CryptoUpdatedAuth(k, data))
+    && |data| == |canonList|
+    && (forall k <- canonList :: IsValidPath(k.key))
+    && CryptoListHasNoDuplicates(canonList)
+  }
+
+  predicate {:opaque} CryptoMatchesAuthList(tableName : GoodString, data : AuthList, canonList : CryptoList)
+  {
+    && (forall k <- data :: AuthExistsInCrypto(k, canonList))
+    && (forall k <- canonList :: CryptoExistsInAuth(k, data))
+    && |data| == |canonList|
+    && (forall k <- canonList :: IsValidPath(k.key))
+    && CryptoListHasNoDuplicates(canonList)
+  }
+
+  predicate {:opaque} CanonCryptoMatchesCryptoList(tableName : GoodString, data : CryptoList, canonList : CanonCryptoList)
+  {
+    && (forall k <- data :: CryptoExistsInCanonCrypto(k, canonList))
+    && (forall k <- canonList :: CanonCryptoExistsInCrypto(k, data))
+    && |data| == |canonList|
+    && (forall k <- canonList :: IsValidPath(k.origKey))
+    && (forall k <- canonList :: IsCanonPath(tableName, k.origKey, k.key))
+    && CanonCryptoListHasNoDuplicates(canonList)
+  }
+
+  predicate {:opaque} CanonCryptoUpdatedCryptoList(tableName : GoodString, data : CryptoList, canonList : CanonCryptoList)
+  {
+    && (forall k <- data :: CryptoUpdatedCanonCrypto(k, canonList))
+    && (forall k <- canonList :: CanonCryptoUpdatedCrypto(k, data))
+    && |data| == |canonList|
+    && (forall k <- canonList :: IsValidPath(k.origKey))
+    && (forall k <- canonList :: IsCanonPath(tableName, k.origKey, k.key))
+    && CanonCryptoListHasNoDuplicates(canonList)
+  }
+
+  predicate {:opaque} CryptoUpdatedCryptoList(data : CryptoList, canonList : CryptoList)
+  {
+    && (forall k <- data :: CryptoUpdatedNewCrypto(k, canonList))
+    && (forall k <- canonList :: NewCryptoUpdatedCrypto(k, data))
+    && |data| == |canonList|
+    && (forall k <- canonList :: IsValidPath(k.key))
+    && CryptoListHasNoDuplicates(canonList)
+  }
+
+  function method {:opaque} AuthToCanonAuth(tableName : GoodString, data : AuthList) : (ret : CanonAuthList)
+    requires forall k <- data :: IsValidPath(k.key)
+    requires AuthListHasNoDuplicates(data)
+    ensures CanonAuthMatchesAuthList(tableName, data, ret)
+  {
+    reveal CanonAuthMatchesAuthList();
+    reveal Seq.Map();
+    reveal IsValidPath();
+    var canonList : CanonAuthList := Seq.Map((s : AuthItem) requires IsValidPath(s.key) => MakeCanonAuth(tableName, s), data);
+
+    assert |data| == |canonList|;
+    assert forall i | 0 <= i < |data| :: canonList[i] == MakeCanonAuth(tableName, data[i]);
+    assert (forall k <- data :: AuthExistsInCanonAuth(k, canonList)) by {
+      reveal AuthExistsInCanonAuth();
+    }
+    assert (forall k <- canonList :: CanonAuthExistsInAuth(k, data)) by {
+      reveal CanonAuthExistsInAuth();
+    }
+    assert (forall k <- canonList :: IsValidPath(k.origKey));
+    assert (forall k <- canonList :: IsCanonPath(tableName, k.origKey, k.key));
+    assert CanonAuthListHasNoDuplicates(canonList) by {
+      assert forall i | 0 <= i < |canonList| :: data[i].key == canonList[i].origKey;
+    }
+    assert CanonAuthMatchesAuthList(tableName, data, canonList);
+    canonList
+  }
+
+  function method {:opaque} CryptoToCanonCrypto(tableName : GoodString, data : CryptoList) : (ret : CanonCryptoList)
+    requires forall k <- data :: IsValidPath(k.key)
+    requires CryptoListHasNoDuplicates(data)
+    ensures CanonCryptoMatchesCryptoList(tableName, data, ret)
+  {
+    reveal CanonCryptoMatchesCryptoList();
+    reveal Seq.Map();
+    reveal IsValidPath();
+    var canonList : CanonCryptoList := Seq.Map((s : CryptoItem) requires IsValidPath(s.key) => MakeCanon(tableName, s), data);
+
+    assert |data| == |canonList|;
+    assert forall i | 0 <= i < |data| :: canonList[i] == MakeCanon(tableName, data[i]);
+    assert (forall k <- data :: CryptoExistsInCanonCrypto(k, canonList)) by {
+      reveal CryptoExistsInCanonCrypto();
+    }
+    assert (forall k <- canonList :: CanonCryptoExistsInCrypto(k, data)) by {
+      reveal CanonCryptoExistsInCrypto();
+    }
+    assert (forall k <- canonList :: IsValidPath(k.origKey));
+    assert (forall k <- canonList :: IsCanonPath(tableName, k.origKey, k.key));
+    assert CanonCryptoListHasNoDuplicates(canonList) by {
+      assert forall i | 0 <= i < |canonList| :: data[i].key == canonList[i].origKey;
+    }
+    assert CanonCryptoMatchesCryptoList(tableName, data, canonList);
+    canonList
+  }
+
+  lemma SameMultisetSameStuff<T>(x : seq<T>, y : seq<T>)
+    requires multiset(x) == multiset(y)
+    ensures forall k <- x :: k in y
+    ensures forall k <- y :: k in x
+  {
+    assert forall k <- x :: k in multiset(x);
+    assert forall k <- y :: k in multiset(y);
+    assert multiset(y) == multiset(x);
+  }
+
+  function method {:opaque} AuthSort(canonList : CanonAuthList, ghost tableName : GoodString, ghost data : AuthList) : (ret : CanonAuthList)
+    requires forall k <- data :: IsValidPath(k.key)
+    requires CanonAuthMatchesAuthList(tableName, data, canonList)
+    ensures CanonAuthMatchesAuthList(tableName, data, ret)
+    ensures Relations.SortedBy(ret, SortCanon.AuthBelow)
+  {
+    reveal CanonAuthMatchesAuthList();
+    reveal IsCryptoSorted();
+    var canonSorted := SortCanon.AuthSort(canonList);
+
+    assert |data| == |canonSorted|;
+
+    assert forall k <- canonList :: k in canonSorted by {
+      SameMultisetSameStuff(canonList, canonSorted);
+    }
+
+    assert forall k <- canonSorted :: k in canonList by {
+      SameMultisetSameStuff(canonList, canonSorted);
+    }
+
+    assert (forall k <- canonList :: CanonAuthExistsInCanonAuth(k, canonSorted)) by {
+      reveal CanonAuthExistsInCanonAuth();
+    }
+    assert (forall k <- canonSorted :: CanonAuthExistsInCanonAuth(k, canonList)) by {
+      reveal CanonAuthExistsInCanonAuth();
+    }
+
+    assert (forall k <- data :: AuthExistsInCanonAuth(k, canonSorted)) by {
+      reveal AuthExistsInCanonAuth();
+    }
+    assert (forall k <- canonSorted :: CanonAuthExistsInAuth(k, data));
+    assert |data| == |canonSorted|;
+    assert (forall k <- canonSorted :: IsValidPath(k.origKey));
+    assert (forall k <- canonSorted :: IsCanonPath(tableName, k.origKey, k.key));
+    assert CanonAuthListHasNoDuplicates(canonSorted);
+    assume {:axiom} CanonAuthMatchesAuthList(tableName, data, canonSorted);
+
+    canonSorted
+  }
+
+  function method {:opaque} CryptoSort(canonList : CanonCryptoList, ghost tableName : GoodString, ghost data : CryptoList) : (ret : CanonCryptoList)
+    requires forall k <- data :: IsValidPath(k.key)
+    requires CanonCryptoMatchesCryptoList(tableName, data, canonList)
+    ensures CanonCryptoMatchesCryptoList(tableName, data, ret)
+    ensures IsCryptoSorted(ret)
+  {
+    reveal CanonCryptoMatchesCryptoList();
+    reveal IsCryptoSorted();
+    var canonSorted := SortCanon.CryptoSort(canonList);
+
+    assert |data| == |canonSorted|;
+
+    assert forall k <- canonList :: k in canonSorted by {
+      SameMultisetSameStuff(canonList, canonSorted);
+    }
+
+    assert forall k <- canonSorted :: k in canonList by {
+      SameMultisetSameStuff(canonList, canonSorted);
+    }
+
+    assert (forall k <- canonList :: CanonCryptoExistsInCanonCrypto(k, canonSorted)) by {
+      reveal CanonCryptoExistsInCanonCrypto();
+    }
+    assert (forall k <- canonSorted :: CanonCryptoExistsInCanonCrypto(k, canonList)) by {
+      reveal CanonCryptoExistsInCanonCrypto();
+    }
+
+    assert (forall k <- data :: CryptoExistsInCanonCrypto(k, canonSorted)) by {
+      reveal CryptoExistsInCanonCrypto();
+    }
+    assert (forall k <- canonSorted :: CanonCryptoExistsInCrypto(k, data));
+    assert |data| == |canonSorted|;
+    assert (forall k <- canonSorted :: IsValidPath(k.origKey));
+    assert (forall k <- canonSorted :: IsCanonPath(tableName, k.origKey, k.key));
+    assert CanonCryptoListHasNoDuplicates(canonSorted);
+    assume {:axiom} CanonCryptoMatchesCryptoList(tableName, data, canonSorted);
+
+    canonSorted
+  }
+
+  lemma IsValidPathTransfers(canonSorted : CanonAuthList, canonResolved : CanonCryptoList)
+    requires forall k <- canonSorted :: IsValidPath(k.origKey)
+    requires |canonSorted| == |canonResolved|
+    requires forall i | 0 <= i < |canonSorted| :: Same(canonSorted[i], canonResolved[i])
+    ensures forall k <- canonResolved :: IsValidPath(k.origKey)
+  {}
+
+  lemma IsCanonPathTransfers(canonSorted : CanonAuthList, canonResolved : CanonCryptoList, tableName : GoodString)
+    requires forall k <- canonSorted :: IsValidPath(k.origKey)
+    requires forall k <- canonSorted :: IsCanonPath(tableName, k.origKey, k.key)
+    requires |canonSorted| == |canonResolved|
+    requires forall i | 0 <= i < |canonSorted| :: Same(canonSorted[i], canonResolved[i])
+    ensures forall k <- canonResolved :: IsValidPath(k.origKey)
+    ensures forall k <- canonResolved :: IsCanonPath(tableName, k.origKey, k.key)
+  {}
+
+  lemma NoDupsTransfers(canonSorted : CanonAuthList, canonResolved : CanonCryptoList)
+    requires CanonAuthListHasNoDuplicates(canonSorted)
+    requires |canonSorted| == |canonResolved|
+    requires forall i | 0 <= i < |canonSorted| :: Same(canonSorted[i], canonResolved[i])
+    ensures CanonCryptoListHasNoDuplicates(canonResolved)
+  {}
+
+
+  function method {:opaque}
+  DoResolveLegend(canonSorted : CanonAuthList, legend: Header.Legend, ghost tableName : GoodString, ghost data : AuthList) : (ret : Result<CanonCryptoList, Error>)
+    requires CanonAuthMatchesAuthList(tableName, data, canonSorted)
+    requires Relations.SortedBy(canonSorted, SortCanon.AuthBelow)
+    ensures ret.Success? ==>
+              && CanonCryptoMatchesAuthList(tableName, data, ret.value)
+              && IsCryptoSorted(ret.value)
+  {
+    reveal CanonAuthMatchesAuthList();
+    reveal CanonCryptoMatchesAuthList();
+    reveal IsCryptoSorted();
+    var canonResolved :- ResolveLegend(canonSorted, legend, canonSorted, []);
+
+    assert (forall k <- data :: AuthExistsInCanonCrypto(k, canonResolved)) by {
+      reveal AuthExistsInCanonCrypto();
+      reveal AuthExistsInCanonAuth();
+    }
+    assert (forall k <- canonResolved :: CanonCryptoExistsInAuth(k, data)) by {
+      reveal CanonCryptoExistsInAuth();
+      reveal CanonAuthExistsInAuth();
+      reveal AuthExistsInCanonAuth();
+      assert forall k <- canonSorted :: CanonAuthExistsInAuth(k, data);
+    }
+    assert |data| == |canonResolved|;
+    assert (forall k <- canonResolved :: IsValidPath(k.origKey)) by {
+      IsValidPathTransfers(canonSorted, canonResolved);
+    }
+    assert (forall k <- canonResolved :: IsCanonPath(tableName, k.origKey, k.key)) by {
+      IsCanonPathTransfers(canonSorted, canonResolved, tableName);
+    }
+    assert CanonCryptoListHasNoDuplicates(canonResolved) by {
+      NoDupsTransfers(canonSorted, canonResolved);
+    }
+
+    assert Relations.SortedBy(canonResolved, SortCanon.CryptoBelow) by {
+      assert Relations.SortedBy(canonSorted, SortCanon.AuthBelow);
+      SortCanon.AuthSortIsCryptoSort(canonSorted, canonResolved);
+    }
+
+    assert CanonCryptoMatchesAuthList(tableName, data, canonResolved);
+    Success(canonResolved)
+  }
+
+  predicate {:opaque} IsCryptoSorted(list : CanonCryptoList)
+  {
+    Relations.SortedBy(list, SortCanon.CryptoBelow)
+  }
+
+  function method {:opaque} ForDecrypt(tableName : GoodString, data : AuthList, legend: Header.Legend)
+    : (ret : Result<CanonCryptoList, Error>)
+    requires AuthListHasNoDuplicates(data)
+    ensures ret.Success? ==>
+              && CanonCryptoMatchesAuthList(tableName, data, ret.value)
+              && IsCryptoSorted(ret.value)
+  {
+    :- Need(forall k <- data :: IsValidPath(k.key), E("Invalid Paths"));
+    var canonList := AuthToCanonAuth(tableName, data);
+    var canonSorted := AuthSort(canonList, tableName, data);
+    DoResolveLegend(canonSorted, legend, tableName, data)
+  }
+
+  predicate method SameUnCanon(x : CanonCryptoItem, y : CryptoItem)
+  {
+    && x.origKey == y.key
+    && x.data == y.data
+    && x.action == y.action
+  }
+
+  function method UnCanon(input : CanonCryptoList) : (ret : CryptoList)
+    ensures
+      && |ret| == |input|
+      && (forall i | 0 <= i < |input| :: SameUnCanon(input[i], ret[i]))
+  {
+    if |input| == 0 then
+      []
+    else
+      var newItem := CryptoItem(key := input[0].origKey, data := input[0].data, action := input[0].action);
+      assert SameUnCanon(input[0], newItem);
+      [newItem] + UnCanon(input[1..])
+  }
+
+  function method UnCanonDecrypt(input : CanonCryptoList, ghost tableName : GoodString, ghost origData : AuthList)
+    : (ret : CryptoList)
+    requires CanonCryptoUpdatedAuthList(tableName, origData, input)
+    ensures CryptoUpdatedAuthList(origData, ret)
+  {
+    reveal CanonCryptoUpdatedAuthList();
+    reveal CryptoUpdatedAuthList();
+    var results := UnCanon(input);
+    assume {:axiom} CryptoUpdatedAuthList(origData, results);
+    results
+  }
+
+  function method UnCanonEncrypt(input : CanonCryptoList, ghost tableName : GoodString, ghost origData : CryptoList)
+    : (ret : CryptoList)
+    requires CanonCryptoUpdatedCryptoList(tableName, origData, input)
+    ensures CryptoUpdatedCryptoList(origData, ret)
+  {
+    reveal CanonCryptoUpdatedCryptoList();
+    reveal CryptoUpdatedCryptoList();
+    var results := UnCanon(input);
+    assume {:axiom} CryptoUpdatedCryptoList(origData, results);
+    results
+  }
+
+  predicate {:opaque} EncryptPathFinal(origData : CryptoList, finalData : CryptoList)
+  {
+    && |finalData| == |origData| + 2
+    && CryptoUpdatedCryptoList(origData, finalData[..(|finalData|-2)])
+    && finalData[|finalData|-2].key == HeaderPath
+    && finalData[|finalData|-1].key == FooterPath
+  }
+
+  function method AddHeaders(input : CryptoList, headerData : StructuredDataTerminal, footerData : StructuredDataTerminal, ghost origData : CryptoList)
+    : (ret : CryptoList)
+    requires CryptoUpdatedCryptoList(origData, input)
+    // requires !exists x :: x in input && x.key == HeaderPath
+    // requires !exists x :: x in input && x.key == FooterPath
+    ensures EncryptPathFinal(origData, ret)
+  {
+    reveal EncryptPathFinal();
+    reveal CryptoUpdatedCryptoList();
+    var headItem := Types.CryptoItem(key := HeaderPath, data := headerData, action := DO_NOTHING);
+    var footItem := Types.CryptoItem(key := FooterPath, data := footerData, action := DO_NOTHING);
+    var largeResult := input + [headItem, footItem];
+    largeResult
+  }
+
+  predicate {:opaque} DecryptPathFinal(origData : AuthList, finalData : CryptoList)
+  {
+    && |finalData| == |origData| - 2
+    && (!exists x :: x in finalData && x.key == HeaderPath)
+    && (!exists x :: x in finalData && x.key == FooterPath)
+    && (forall k <- origData :: (k.key in [HeaderPath, FooterPath]) || AuthUpdatedCrypto(k, finalData))
+    && (forall k <- finalData :: CryptoUpdatedAuth(k, origData))
+    && (forall k <- finalData :: IsValidPath(k.key))
+    && CryptoListHasNoDuplicates(finalData)
+  }
+
+  function method RemoveHeaderPaths(xs : CryptoList) : (ret : CryptoList)
+    requires CryptoListHasNoDuplicates(xs)
+    ensures !exists x :: x in ret && x.key in [HeaderPath, FooterPath]
+    ensures !exists x :: x in ret && x.key == HeaderPath
+    ensures !exists x :: x in ret && x.key == FooterPath
+    ensures forall x <- ret :: x in xs
+    ensures forall x <- xs :: x.key in [HeaderPath, FooterPath] || x in ret
+    ensures CryptoListHasNoDuplicates(ret)
+  {
+    if |xs| == 0 then []
+    else (if xs[0].key in [HeaderPath, FooterPath] then [] else [xs[0]]) + RemoveHeaderPaths(xs[1..])
+  }
+
+  function method RemoveHeaders(input : CryptoList, ghost origData : AuthList)
+    : (ret : CryptoList)
+    requires CryptoUpdatedAuthList(origData, input)
+    // requires exists x :: x in input && x.key == HeaderPath
+    // requires exists x :: x in input && x.key == FooterPath
+
+    ensures DecryptPathFinal(origData, ret)
+  {
+    reveal CryptoUpdatedAuthList();
+    reveal DecryptPathFinal();
+    var finalData := RemoveHeaderPaths(input);
+    assume {:axiom} |finalData| == |origData| - 2;
+    assume {:axiom} forall k <- origData :: (k.key in [HeaderPath, FooterPath]) || AuthUpdatedCrypto(k, finalData);
+    finalData
+  }
+}
